aspec+capDL: refactor VMAttributes_A
- Refactor VMAttributes_A into an ASpec and a capDL part, because only
  capDL needs the validation definitions. Avoid requalifying any of the
  virtual memory attribute constants and types in ASpec to keep generic
  code fully agnostic. Instead, requalify only in capDL where all of
  these constants are currently used by a unified spec between ARM and
  ARM_HYP.

- Add AARCH64 instance of these definitions.

Signed-off-by: Gerwin Klein <gerwin.klein@proofcraft.systems>

spec/abstract/AARCH64/ArchVMAttributes_A.thy
@@ -1,5 +1,5 @@
 (*
- * Copyright 2014, General Dynamics C4 Systems
+ * Copyright 2022, Proofcraft Pty Ltd
  *
  * SPDX-License-Identifier: GPL-2.0-only
  *)
@@ -15,20 +15,28 @@ context Arch begin arch_global_naming (A)
 
 (* Union of attributes and non-seL4 rights that the kernel uses on pages and page tables,
    including kernel-only attributes. Not all are reachable via attribs_from_word. *)
-datatype vm_attribute = PageCacheable | XNever
+datatype vm_attribute = Global | Execute | Device
 type_synonym vm_attributes = "vm_attribute set"
 
 type_synonym arch_raw_vmattrs = machine_word
 
 definition attribs_from_word :: "machine_word \<Rightarrow> vm_attributes" where
-  "attribs_from_word w \<equiv>
-     let V = (if w !! 0 then {PageCacheable} else {})
-     in if w !! 2 then insert XNever V else V"
+  "attribs_from_word w \<equiv> {attr. \<not>w !! 0 \<and> attr = Device \<or> \<not>w !! 2 \<and> attr = Execute}"
 
 definition attribs_to_word :: "vm_attributes \<Rightarrow> machine_word" where
   "attribs_to_word attribs \<equiv>
-     let V = (if PageCacheable \<in> attribs then 1 else 0)
-     in if XNever \<in> attribs then V + 4 else V "
+     let V = (if Device \<in> attribs then 0 else 1);
+         V' = (if Execute \<in> attribs then V else V + 4)
+     in V'"
+
+(* sanity check *)
+lemma attribs_from_to_word:
+  "attribs_from_word (attribs_to_word A) = A - {Global}"
+  unfolding attribs_from_word_def attribs_to_word_def
+  using vm_attribute.exhaust
+  by clarsimp
+     blast
 
 end
+
 end
