spec/abstract/ARM/ArchVMAttributes_A.thy
@@ -22,28 +22,15 @@ type_synonym arch_raw_vmattrs = machine_word
 
 definition attribs_from_word :: "machine_word \<Rightarrow> vm_attributes" where
   "attribs_from_word w \<equiv>
-     let V = (if w !!0 then {PageCacheable} else {});
-         V' = (if w!!1 then insert ParityEnabled V else V)
-     in if w!!2 then insert XNever V' else V'"
+     let V = (if w !! 0 then {PageCacheable} else {});
+         V' = (if w !! 1 then insert ParityEnabled V else V)
+     in if w !! 2 then insert XNever V' else V'"
 
 definition attribs_to_word :: "vm_attributes \<Rightarrow> machine_word" where
   "attribs_to_word attribs \<equiv>
      let V = (if PageCacheable \<in> attribs then 1 else 0);
          V' = (if ParityEnabled \<in> attribs then V + 2 else V)
      in if XNever \<in> attribs then V' + 4 else V' "
-
-definition validate_vm_attributes :: "machine_word \<Rightarrow> vmpage_size \<Rightarrow> machine_word"  where
-  "validate_vm_attributes attr sz \<equiv> case sz of
-     ARM.ARMSmallPage \<Rightarrow> attribs_to_word (attribs_from_word attr - {Global, ParityEnabled})
-   | ARM.ARMLargePage \<Rightarrow> attribs_to_word (attribs_from_word attr - {Global, ParityEnabled})
-   | ARM.ARMSection \<Rightarrow> attribs_to_word (attribs_from_word attr - {Global})
-   | ARM.ARMSuperSection \<Rightarrow> attribs_to_word (attribs_from_word attr - {Global})"
-
-definition validate_pt_vm_attributes :: "machine_word \<Rightarrow> machine_word"  where
-  "validate_pt_vm_attributes attr \<equiv> attribs_to_word (attribs_from_word attr \<inter> {ParityEnabled})"
-
-definition default_vmattrs :: "machine_word" where
-  "default_vmattrs \<equiv> 3"
 
 end
 end
