spec/capDL/ARM/ArchVMAttributes_D.thy
@@ -1,0 +1,37 @@
+(*
+ * Copyright 2014, General Dynamics C4 Systems
+ *
+ * SPDX-License-Identifier: GPL-2.0-only
+ *)
+
+(* Definition of architecture-dependent VM attribute validation. *)
+
+theory ArchVMAttributes_D
+imports
+  ASpec.ArchVMAttributes_A
+begin
+
+context Arch begin arch_global_naming (A)
+
+definition validate_vm_attributes :: "machine_word \<Rightarrow> vmpage_size \<Rightarrow> machine_word"  where
+  "validate_vm_attributes attr sz \<equiv> case sz of
+     ARMSmallPage \<Rightarrow> attribs_to_word (attribs_from_word attr - {Global, ParityEnabled})
+   | ARMLargePage \<Rightarrow> attribs_to_word (attribs_from_word attr - {Global, ParityEnabled})
+   | ARMSection \<Rightarrow> attribs_to_word (attribs_from_word attr - {Global})
+   | ARMSuperSection \<Rightarrow> attribs_to_word (attribs_from_word attr - {Global})"
+
+definition validate_pt_vm_attributes :: "machine_word \<Rightarrow> machine_word"  where
+  "validate_pt_vm_attributes attr \<equiv> attribs_to_word (attribs_from_word attr \<inter> {ParityEnabled})"
+
+lemma validate_vm_attributes_0[simp]:
+  "validate_vm_attributes 0 vmsz = 0"
+  unfolding validate_vm_attributes_def
+  by (clarsimp simp: attribs_from_word_def attribs_to_word_def split: vmpage_size.splits)
+
+lemma validate_pt_vm_attributes_0[simp]:
+  "validate_pt_vm_attributes 0 = 0"
+  unfolding validate_pt_vm_attributes_def
+  by (simp add: attribs_from_word_def attribs_to_word_def)
+
+end
+end
